<?xml version="1.0"?>
<rdf:RDF xmlns="http://www.semanticweb.org/yasen/ontologies/2024/5/uml/"
     xml:base="http://www.semanticweb.org/yasen/ontologies/2024/5/uml/"
     xmlns:owl="http://www.w3.org/2002/07/owl#"
     xmlns:rdf="http://www.w3.org/1999/02/22-rdf-syntax-ns#"
     xmlns:xml="http://www.w3.org/XML/1998/namespace"
     xmlns:xsd="http://www.w3.org/2001/XMLSchema#"
     xmlns:rdfs="http://www.w3.org/2000/01/rdf-schema#">
    <owl:Ontology rdf:about="http://www.semanticweb.org/yasen/ontologies/2024/5/uml">
        <rdfs:comment>Reference: https://www.uml-diagrams.org/uml-25-diagrams.html</rdfs:comment>
        <rdfs:comment>UML Specification v2.5.1: https://www.omg.org/spec/UML/2.5.1/About-UML/</rdfs:comment>
    </owl:Ontology>
    


    <!-- 
    ///////////////////////////////////////////////////////////////////////////////////////
    //
    // Classes
    //
    ///////////////////////////////////////////////////////////////////////////////////////
     -->

    


    <!-- http://www.semanticweb.org/yasen/ontologies/2024/5/uml#Actions -->

    <owl:Class rdf:about="http://www.semanticweb.org/yasen/ontologies/2024/5/uml#Actions">
        <rdfs:subClassOf rdf:resource="http://www.semanticweb.org/yasen/ontologies/2024/5/uml#Behavioral_Modeling"/>
    </owl:Class>
    


    <!-- http://www.semanticweb.org/yasen/ontologies/2024/5/uml#Activities -->

    <owl:Class rdf:about="http://www.semanticweb.org/yasen/ontologies/2024/5/uml#Activities">
        <rdfs:subClassOf rdf:resource="http://www.semanticweb.org/yasen/ontologies/2024/5/uml#Behavioral_Modeling"/>
    </owl:Class>
    


    <!-- http://www.semanticweb.org/yasen/ontologies/2024/5/uml#Activity_Diagram -->

    <owl:Class rdf:about="http://www.semanticweb.org/yasen/ontologies/2024/5/uml#Activity_Diagram">
        <rdfs:subClassOf rdf:resource="http://www.semanticweb.org/yasen/ontologies/2024/5/uml#Behavioral_Diagrams"/>
        <rdfs:comment>Shows sequence and conditions for coordinating lower-level behaviors, rather than which classifiers own those behaviors. These are commonly called control flow and object flow models.</rdfs:comment>
    </owl:Class>
    


    <!-- http://www.semanticweb.org/yasen/ontologies/2024/5/uml#Behavioral_Diagrams -->

    <owl:Class rdf:about="http://www.semanticweb.org/yasen/ontologies/2024/5/uml#Behavioral_Diagrams">
        <rdfs:subClassOf rdf:resource="http://www.semanticweb.org/yasen/ontologies/2024/5/uml#Diagram_Classification"/>
        <rdfs:comment>Behavior diagrams show the dynamic behavior of the objects in a system, which can be described as a series of changes to the system over time.</rdfs:comment>
        <rdfs:seeAlso>Dynamic UML Modeling</rdfs:seeAlso>
    </owl:Class>
    


    <!-- http://www.semanticweb.org/yasen/ontologies/2024/5/uml#Behavioral_Modeling -->

    <owl:Class rdf:about="http://www.semanticweb.org/yasen/ontologies/2024/5/uml#Behavioral_Modeling">
        <rdfs:subClassOf rdf:resource="http://www.semanticweb.org/yasen/ontologies/2024/5/uml#Semantic_Areas"/>
        <rdfs:comment>The base behavioral semantics of UML builds on this structural foundation to provide a basic framework for the execution of behaviors.</rdfs:comment>
    </owl:Class>
    


    <!-- http://www.semanticweb.org/yasen/ontologies/2024/5/uml#Behavioral_State_Machine_DIagram -->

    <owl:Class rdf:about="http://www.semanticweb.org/yasen/ontologies/2024/5/uml#Behavioral_State_Machine_DIagram">
        <rdfs:subClassOf rdf:resource="http://www.semanticweb.org/yasen/ontologies/2024/5/uml#State_Machine_Diagram"/>
        <rdfs:comment>Shows discrete behavior of a part of designed system through finite state transitions.</rdfs:comment>
    </owl:Class>
    


    <!-- http://www.semanticweb.org/yasen/ontologies/2024/5/uml#Class_Diagram -->

    <owl:Class rdf:about="http://www.semanticweb.org/yasen/ontologies/2024/5/uml#Class_Diagram">
        <rdfs:subClassOf rdf:resource="http://www.semanticweb.org/yasen/ontologies/2024/5/uml#Structural_Diagrams"/>
        <rdfs:comment>Shows structure of the designed system, subsystem or component as related classes and interfaces, with their features, constraints and relationships - associations, generalizations, dependencies, etc.</rdfs:comment>
    </owl:Class>
    


    <!-- http://www.semanticweb.org/yasen/ontologies/2024/5/uml#Classifiers -->

    <owl:Class rdf:about="http://www.semanticweb.org/yasen/ontologies/2024/5/uml#Classifiers">
        <rdfs:subClassOf rdf:resource="http://www.semanticweb.org/yasen/ontologies/2024/5/uml#Structural_Modeling"/>
    </owl:Class>
    


    <!-- http://www.semanticweb.org/yasen/ontologies/2024/5/uml#Collaboration_Use_Diagram -->

    <owl:Class rdf:about="http://www.semanticweb.org/yasen/ontologies/2024/5/uml#Collaboration_Use_Diagram">
        <rdfs:subClassOf rdf:resource="http://www.semanticweb.org/yasen/ontologies/2024/5/uml#Composite_Structure_Diagram"/>
        <rdfs:comment>Shows objects in a system cooperating with each other to produce some behavior of the system.</rdfs:comment>
    </owl:Class>
    


    <!-- http://www.semanticweb.org/yasen/ontologies/2024/5/uml#Common_Behavior -->

    <owl:Class rdf:about="http://www.semanticweb.org/yasen/ontologies/2024/5/uml#Common_Behavior">
        <rdfs:subClassOf rdf:resource="http://www.semanticweb.org/yasen/ontologies/2024/5/uml#Behavioral_Modeling"/>
    </owl:Class>
    


    <!-- http://www.semanticweb.org/yasen/ontologies/2024/5/uml#Common_Structure -->

    <owl:Class rdf:about="http://www.semanticweb.org/yasen/ontologies/2024/5/uml#Common_Structure">
        <rdfs:subClassOf rdf:resource="http://www.semanticweb.org/yasen/ontologies/2024/5/uml#Structural_Modeling"/>
    </owl:Class>
    


    <!-- http://www.semanticweb.org/yasen/ontologies/2024/5/uml#Communication_Diagram -->

    <owl:Class rdf:about="http://www.semanticweb.org/yasen/ontologies/2024/5/uml#Communication_Diagram">
        <rdfs:subClassOf rdf:resource="http://www.semanticweb.org/yasen/ontologies/2024/5/uml#Interaction_Diagram"/>
        <rdfs:comment>Focuses on the interaction between lifelines where the architecture of the internal structure and how this corresponds with the message passing is central. The sequencing of messages is given through a sequence numbering scheme.</rdfs:comment>
        <owl:deprecated>a.k.a. Collaboration diagram in UML 1.x</owl:deprecated>
    </owl:Class>
    


    <!-- http://www.semanticweb.org/yasen/ontologies/2024/5/uml#Component_Diagram -->

    <owl:Class rdf:about="http://www.semanticweb.org/yasen/ontologies/2024/5/uml#Component_Diagram">
        <rdfs:subClassOf rdf:resource="http://www.semanticweb.org/yasen/ontologies/2024/5/uml#Structural_Diagrams"/>
        <rdfs:comment>Shows components and dependencies between them. This type of diagrams is used for Component-Based Development (CBD), to describe systems with Service-Oriented Architecture (SOA).</rdfs:comment>
    </owl:Class>
    


    <!-- http://www.semanticweb.org/yasen/ontologies/2024/5/uml#Composite_Structure_Diagram -->

    <owl:Class rdf:about="http://www.semanticweb.org/yasen/ontologies/2024/5/uml#Composite_Structure_Diagram">
        <rdfs:subClassOf rdf:resource="http://www.semanticweb.org/yasen/ontologies/2024/5/uml#Structural_Diagrams"/>
        <rdfs:comment>Diagram could be used to show:
- Internal structure of a classifier
- A behavior of a collaboration</rdfs:comment>
    </owl:Class>
    


    <!-- http://www.semanticweb.org/yasen/ontologies/2024/5/uml#Deployment_Diagram -->

    <owl:Class rdf:about="http://www.semanticweb.org/yasen/ontologies/2024/5/uml#Deployment_Diagram">
        <rdfs:subClassOf rdf:resource="http://www.semanticweb.org/yasen/ontologies/2024/5/uml#Structural_Diagrams"/>
        <rdfs:comment>Shows architecture of the system as deployment (distribution) of software artifacts to deployment targets.
Note, that components were directly deployed to nodes in UML 1.x deployment diagrams. In UML 2.x artifacts are deployed to nodes, and artifacts could manifest (implement) components. Components are deployed to nodes indirectly through artifacts.

Specification level deployment diagram (also called type level) shows some overview of deployment of artifacts to deployment targets, without referencing specific instances of artifacts or nodes.

Instance level deployment diagram shows deployment of instances of artifacts to specific instances of deployment targets. It could be used for example to show differences in deployments to development, staging or production environments with the names/ids of specific build or deployment servers or devices.</rdfs:comment>
    </owl:Class>
    


    <!-- http://www.semanticweb.org/yasen/ontologies/2024/5/uml#Deployments -->

    <owl:Class rdf:about="http://www.semanticweb.org/yasen/ontologies/2024/5/uml#Deployments">
        <rdfs:subClassOf rdf:resource="http://www.semanticweb.org/yasen/ontologies/2024/5/uml#Supplemental_Modeling"/>
    </owl:Class>
    


    <!-- http://www.semanticweb.org/yasen/ontologies/2024/5/uml#Diagram_Classification -->

    <owl:Class rdf:about="http://www.semanticweb.org/yasen/ontologies/2024/5/uml#Diagram_Classification">
        <rdfs:comment>V2 grouping based on https://www.uml-diagrams.org/uml-25-diagrams.html</rdfs:comment>
    </owl:Class>
    


    <!-- http://www.semanticweb.org/yasen/ontologies/2024/5/uml#Information_Flow_Diagram -->

    <owl:Class rdf:about="http://www.semanticweb.org/yasen/ontologies/2024/5/uml#Information_Flow_Diagram">
        <rdfs:subClassOf rdf:resource="http://www.semanticweb.org/yasen/ontologies/2024/5/uml#Behavioral_Diagrams"/>
        <rdfs:subClassOf rdf:resource="http://www.semanticweb.org/yasen/ontologies/2024/5/uml#Class_Diagram"/>
        <rdfs:comment>Shows exchange of information between system entities at some high levels of abstraction. Information flows may be useful to describe circulation of information through a system by representing aspects of models not yet fully specified or with less details.</rdfs:comment>
    </owl:Class>
    


    <!-- http://www.semanticweb.org/yasen/ontologies/2024/5/uml#Information_Flows -->

    <owl:Class rdf:about="http://www.semanticweb.org/yasen/ontologies/2024/5/uml#Information_Flows">
        <rdfs:subClassOf rdf:resource="http://www.semanticweb.org/yasen/ontologies/2024/5/uml#Supplemental_Modeling"/>
    </owl:Class>
    


    <!-- http://www.semanticweb.org/yasen/ontologies/2024/5/uml#Interaction_Diagram -->

    <owl:Class rdf:about="http://www.semanticweb.org/yasen/ontologies/2024/5/uml#Interaction_Diagram">
        <rdfs:subClassOf rdf:resource="http://www.semanticweb.org/yasen/ontologies/2024/5/uml#Behavioral_Diagrams"/>
        <rdfs:comment>Interaction diagrams include several different types of diagrams:
- sequence diagrams,
- communication diagrams (known as collaboration diagrams in UML 1.x),
- timing diagrams,
- interaction overview diagrams.</rdfs:comment>
    </owl:Class>
    


    <!-- http://www.semanticweb.org/yasen/ontologies/2024/5/uml#Interaction_Overview_Diagram -->

    <owl:Class rdf:about="http://www.semanticweb.org/yasen/ontologies/2024/5/uml#Interaction_Overview_Diagram">
        <rdfs:subClassOf rdf:resource="http://www.semanticweb.org/yasen/ontologies/2024/5/uml#Activity_Diagram"/>
        <rdfs:subClassOf rdf:resource="http://www.semanticweb.org/yasen/ontologies/2024/5/uml#Interaction_Diagram"/>
        <owl:deprecated>Defines interactions through a variant of activity diagrams in a way that promotes overview of the control flow. Interaction overview diagrams focus on the overview of the flow of control where the nodes are interactions or interaction uses. The lifelines and the messages do not appear at this overview level.</owl:deprecated>
    </owl:Class>
    


    <!-- http://www.semanticweb.org/yasen/ontologies/2024/5/uml#Interactions -->

    <owl:Class rdf:about="http://www.semanticweb.org/yasen/ontologies/2024/5/uml#Interactions">
        <rdfs:subClassOf rdf:resource="http://www.semanticweb.org/yasen/ontologies/2024/5/uml#Behavioral_Modeling"/>
    </owl:Class>
    


    <!-- http://www.semanticweb.org/yasen/ontologies/2024/5/uml#Internal_Structure_Diagram -->

    <owl:Class rdf:about="http://www.semanticweb.org/yasen/ontologies/2024/5/uml#Internal_Structure_Diagram">
        <rdfs:subClassOf rdf:resource="http://www.semanticweb.org/yasen/ontologies/2024/5/uml#Composite_Structure_Diagram"/>
        <rdfs:comment>Shows internal structure of a classifier - a decomposition of the classifier into its properties, parts and relationships.</rdfs:comment>
    </owl:Class>
    


    <!-- http://www.semanticweb.org/yasen/ontologies/2024/5/uml#Mainfestation_Diagram -->

    <owl:Class rdf:about="http://www.semanticweb.org/yasen/ontologies/2024/5/uml#Mainfestation_Diagram">
        <rdfs:subClassOf rdf:resource="http://www.semanticweb.org/yasen/ontologies/2024/5/uml#Component_Diagram"/>
        <rdfs:subClassOf rdf:resource="http://www.semanticweb.org/yasen/ontologies/2024/5/uml#Deployment_Diagram"/>
        <rdfs:comment>While component diagrams show components and relationships between components and classifiers, and deployment diagrams - deployments of artifacts to deployment targets, some missing intermediate diagram is manifestation diagram to be used to show manifestation (implementation) of components by artifacts and internal structure of artifacts.
Because manifestation diagrams are not defined by UML 2.5 specification, manifestation of components by artifacts could be shown using either component diagrams or deployment diagrams.</rdfs:comment>
    </owl:Class>
    


    <!-- http://www.semanticweb.org/yasen/ontologies/2024/5/uml#Model_Diagram -->

    <owl:Class rdf:about="http://www.semanticweb.org/yasen/ontologies/2024/5/uml#Model_Diagram">
        <rdfs:subClassOf rdf:resource="http://www.semanticweb.org/yasen/ontologies/2024/5/uml#Package_Diagram"/>
        <rdfs:comment>UML auxiliary structure diagram which shows some abstraction or specific view of a system, to describe architectural, logical or behavioral aspects of the system. It could show, for example, architecture of a multi-layered (aka multi-tiered) application - see multi-layered application model.</rdfs:comment>
    </owl:Class>
    


    <!-- http://www.semanticweb.org/yasen/ontologies/2024/5/uml#Network_Architecture_Diagram -->

    <owl:Class rdf:about="http://www.semanticweb.org/yasen/ontologies/2024/5/uml#Network_Architecture_Diagram">
        <rdfs:subClassOf rdf:resource="http://www.semanticweb.org/yasen/ontologies/2024/5/uml#Deployment_Diagram"/>
        <rdfs:comment>Deployment diagrams could be used to show logical or physical network architecture of the system. This kind of deployment diagrams - not formally defined in UML 2.5 - could be called network architecture diagrams.</rdfs:comment>
    </owl:Class>
    


    <!-- http://www.semanticweb.org/yasen/ontologies/2024/5/uml#Object_Diagram -->

    <owl:Class rdf:about="http://www.semanticweb.org/yasen/ontologies/2024/5/uml#Object_Diagram">
        <rdfs:subClassOf rdf:resource="http://www.semanticweb.org/yasen/ontologies/2024/5/uml#Structural_Diagrams"/>
        <rdfs:comment>Instance level class diagram which shows instance specifications of classes and interfaces (objects), slots with value specifications, and links (instances of association).

Object diagram was defined in now obsolete UML 1.4.2 Specification as &quot;a graph of instances, including objects and data values. A static object diagram is an instance of a class diagram; it shows a snapshot of the detailed state of a system at a point in time.&quot; It also stated that object diagram is &quot;a class diagram with objects and no classes.&quot;</rdfs:comment>
    </owl:Class>
    


    <!-- http://www.semanticweb.org/yasen/ontologies/2024/5/uml#Package_Diagram -->

    <owl:Class rdf:about="http://www.semanticweb.org/yasen/ontologies/2024/5/uml#Package_Diagram">
        <rdfs:subClassOf rdf:resource="http://www.semanticweb.org/yasen/ontologies/2024/5/uml#Structural_Diagrams"/>
        <rdfs:comment>Shows packages and relationships between the packages.</rdfs:comment>
    </owl:Class>
    


    <!-- http://www.semanticweb.org/yasen/ontologies/2024/5/uml#Packages -->

    <owl:Class rdf:about="http://www.semanticweb.org/yasen/ontologies/2024/5/uml#Packages">
        <rdfs:subClassOf rdf:resource="http://www.semanticweb.org/yasen/ontologies/2024/5/uml#Structural_Modeling"/>
    </owl:Class>
    


    <!-- http://www.semanticweb.org/yasen/ontologies/2024/5/uml#Profile_Diagram -->

    <owl:Class rdf:about="http://www.semanticweb.org/yasen/ontologies/2024/5/uml#Profile_Diagram">
        <rdfs:subClassOf rdf:resource="http://www.semanticweb.org/yasen/ontologies/2024/5/uml#Structural_Diagrams"/>
        <rdfs:comment>Auxiliary UML diagram which allows to define custom stereotypes, tagged values, and constraints as a lightweight extension mechanism to the UML standard. Profiles allow to adapt the UML metamodel for different
- platforms (such as J2EE or .NET), or
- domains (such as real-time or business process modeling).
Profile diagrams were first introduced in UML 2.0.</rdfs:comment>
    </owl:Class>
    


    <!-- http://www.semanticweb.org/yasen/ontologies/2024/5/uml#Protocol_State_Machine_Diagram -->

    <owl:Class rdf:about="http://www.semanticweb.org/yasen/ontologies/2024/5/uml#Protocol_State_Machine_Diagram">
        <rdfs:subClassOf rdf:resource="http://www.semanticweb.org/yasen/ontologies/2024/5/uml#Behavioral_State_Machine_DIagram"/>
        <rdfs:comment>Shows usage protocol or a lifecycle of some classifier, e.g. which operations of the classifier may be called in each state of the classifier, under which specific conditions, and satisfying some optional postconditions after the classifier transitions to a target state.</rdfs:comment>
    </owl:Class>
    


    <!-- http://www.semanticweb.org/yasen/ontologies/2024/5/uml#Semantic_Areas -->

    <owl:Class rdf:about="http://www.semanticweb.org/yasen/ontologies/2024/5/uml#Semantic_Areas"/>
    


    <!-- http://www.semanticweb.org/yasen/ontologies/2024/5/uml#Sequence_Diagram -->

    <owl:Class rdf:about="http://www.semanticweb.org/yasen/ontologies/2024/5/uml#Sequence_Diagram">
        <rdfs:subClassOf rdf:resource="http://www.semanticweb.org/yasen/ontologies/2024/5/uml#Interaction_Diagram"/>
        <rdfs:comment>Most common kind of interaction diagrams which focuses on the message interchange between lifelines (objects).</rdfs:comment>
    </owl:Class>
    


    <!-- http://www.semanticweb.org/yasen/ontologies/2024/5/uml#State_Machine_Diagram -->

    <owl:Class rdf:about="http://www.semanticweb.org/yasen/ontologies/2024/5/uml#State_Machine_Diagram">
        <rdfs:subClassOf rdf:resource="http://www.semanticweb.org/yasen/ontologies/2024/5/uml#Behavioral_Diagrams"/>
        <rdfs:comment>Used for modeling discrete behavior through finite state transitions. In addition to expressing the behavior of a part of the system, state machines can also be used to express the usage protocol of part of a system. These two kinds of state machines are referred to as behavioral state machines and protocol state machines.</rdfs:comment>
    </owl:Class>
    


    <!-- http://www.semanticweb.org/yasen/ontologies/2024/5/uml#State_Machines -->

    <owl:Class rdf:about="http://www.semanticweb.org/yasen/ontologies/2024/5/uml#State_Machines">
        <rdfs:subClassOf rdf:resource="http://www.semanticweb.org/yasen/ontologies/2024/5/uml#Behavioral_Modeling"/>
    </owl:Class>
    


    <!-- http://www.semanticweb.org/yasen/ontologies/2024/5/uml#Structural_Diagrams -->

    <owl:Class rdf:about="http://www.semanticweb.org/yasen/ontologies/2024/5/uml#Structural_Diagrams">
        <rdfs:subClassOf rdf:resource="http://www.semanticweb.org/yasen/ontologies/2024/5/uml#Diagram_Classification"/>
        <rdfs:comment>Structure diagrams show static structure of the system and its parts on different abstraction and implementation levels and how those parts are related to each other. The elements in a structure diagram represent the meaningful concepts of a system, and may include abstract, real world and implementation concepts.

Structure diagrams are not utilizing time related concepts, do not show the details of dynamic behavior. However, they may show relationships to the behaviors of the classifiers exhibited in the structure diagrams.</rdfs:comment>
        <rdfs:seeAlso>Static UML Modeling</rdfs:seeAlso>
    </owl:Class>
    


    <!-- http://www.semanticweb.org/yasen/ontologies/2024/5/uml#Structural_Modeling -->

    <owl:Class rdf:about="http://www.semanticweb.org/yasen/ontologies/2024/5/uml#Structural_Modeling">
        <rdfs:subClassOf rdf:resource="http://www.semanticweb.org/yasen/ontologies/2024/5/uml#Semantic_Areas"/>
        <rdfs:comment>The structural semantics of UML provides the foundation for the behavioral semnatics of UML.</rdfs:comment>
    </owl:Class>
    


    <!-- http://www.semanticweb.org/yasen/ontologies/2024/5/uml#Supplemental_Modeling -->

    <owl:Class rdf:about="http://www.semanticweb.org/yasen/ontologies/2024/5/uml#Supplemental_Modeling">
        <rdfs:subClassOf rdf:resource="http://www.semanticweb.org/yasen/ontologies/2024/5/uml#Semantic_Areas"/>
    </owl:Class>
    


    <!-- http://www.semanticweb.org/yasen/ontologies/2024/5/uml#Timing_Diagram -->

    <owl:Class rdf:about="http://www.semanticweb.org/yasen/ontologies/2024/5/uml#Timing_Diagram">
        <rdfs:subClassOf rdf:resource="http://www.semanticweb.org/yasen/ontologies/2024/5/uml#Interaction_Diagram"/>
        <owl:deprecated>Shows interactions when a primary purpose of the diagram is to reason about time. Timing diagrams focus on conditions changing within and among lifelines along a linear time axis.</owl:deprecated>
    </owl:Class>
    


    <!-- http://www.semanticweb.org/yasen/ontologies/2024/5/uml#UseCase_Diagram -->

    <owl:Class rdf:about="http://www.semanticweb.org/yasen/ontologies/2024/5/uml#UseCase_Diagram">
        <rdfs:subClassOf rdf:resource="http://www.semanticweb.org/yasen/ontologies/2024/5/uml#Behavioral_Diagrams"/>
        <rdfs:subClassOf rdf:resource="http://www.semanticweb.org/yasen/ontologies/2024/5/uml#Class_Diagram"/>
        <rdfs:comment>Describes a set of actions (use cases) that some system or systems (subject) should or can perform in collaboration with one or more external users of the system (actors) to provide some observable and valuable results to the actors or other stakeholders of the system(s).</rdfs:comment>
    </owl:Class>
    


    <!-- http://www.semanticweb.org/yasen/ontologies/2024/5/uml#Use_Cases -->

    <owl:Class rdf:about="http://www.semanticweb.org/yasen/ontologies/2024/5/uml#Use_Cases">
        <rdfs:subClassOf rdf:resource="http://www.semanticweb.org/yasen/ontologies/2024/5/uml#Supplemental_Modeling"/>
    </owl:Class>
    


    <!-- http://www.semanticweb.org/yasen/ontologies/2024/5/uml#Values -->

    <owl:Class rdf:about="http://www.semanticweb.org/yasen/ontologies/2024/5/uml#Values">
        <rdfs:subClassOf rdf:resource="http://www.semanticweb.org/yasen/ontologies/2024/5/uml#Structural_Modeling"/>
    </owl:Class>
    


    <!-- 
    ///////////////////////////////////////////////////////////////////////////////////////
    //
    // Annotations
    //
    ///////////////////////////////////////////////////////////////////////////////////////
     -->

    <rdf:Description rdf:about="http://www.w3.org/2002/07/owl#Thing">
        <rdfs:label>UML</rdfs:label>
    </rdf:Description>
</rdf:RDF>



<!-- Generated by the OWL API (version 4.5.29.2024-05-13T12:11:03Z) https://github.com/owlcs/owlapi -->

